ocaml/extracted/extract.v
@@ -141,15 +141,10 @@ From marble Require pqueue.
 From marble Require traverse.
 
 Extraction Inline
-  traverse.srefl
-  traverse.strans
-  traverse.transform
   traverse.visit'
   traverse.hook_pre
   traverse.traverse_pre'
   traverse.hook_post
-  traverse.mrefl
-  traverse.mtrans
   traverse.visit_cps'
 .
 
